(*  Title:      HOLCF/Sprod.thy
    ID:         $Id$
    Author:     Franz Regensburger and Brian Huffman

Strict product with typedef.
*)

header {* The type of strict products *}

theory Sprod
imports Cprod
begin

defaultsort pcpo

subsection {* Definition of strict product type *}

pcpodef (Sprod)  ('a, 'b) "**" (infixr "**" 20) =
        "{p::'a \<times> 'b. p = \<bottom> \<or> (cfst\<cdot>p \<noteq> \<bottom> \<and> csnd\<cdot>p \<noteq> \<bottom>)}"
by simp

syntax (xsymbols)
  "**"		:: "[type, type] => type"	 ("(_ \<otimes>/ _)" [21,20] 20)
syntax (HTML output)
  "**"		:: "[type, type] => type"	 ("(_ \<otimes>/ _)" [21,20] 20)

lemma spair_lemma:
  "<strictify\<cdot>(\<Lambda> b. a)\<cdot>b, strictify\<cdot>(\<Lambda> a. b)\<cdot>a> \<in> Sprod"
by (simp add: Sprod_def strictify_conv_if cpair_strict)

subsection {* Definitions of constants *}

consts
  sfst :: "('a ** 'b) \<rightarrow> 'a"
  ssnd :: "('a ** 'b) \<rightarrow> 'b"
  spair :: "'a \<rightarrow> 'b \<rightarrow> ('a ** 'b)"
  ssplit :: "('a \<rightarrow> 'b \<rightarrow> 'c) \<rightarrow> ('a ** 'b) \<rightarrow> 'c"

defs
  sfst_def: "sfst \<equiv> \<Lambda> p. cfst\<cdot>(Rep_Sprod p)"
  ssnd_def: "ssnd \<equiv> \<Lambda> p. csnd\<cdot>(Rep_Sprod p)"
  spair_def: "spair \<equiv> \<Lambda> a b. Abs_Sprod
                <strictify\<cdot>(\<Lambda> b. a)\<cdot>b, strictify\<cdot>(\<Lambda> a. b)\<cdot>a>"
  ssplit_def: "ssplit \<equiv> \<Lambda> f. strictify\<cdot>(\<Lambda> p. f\<cdot>(sfst\<cdot>p)\<cdot>(ssnd\<cdot>p))"

syntax  
  "@stuple" :: "['a, args] => 'a ** 'b"  ("(1'(:_,/ _:'))")

translations
  "(:x, y, z:)" == "(:x, (:y, z:):)"
  "(:x, y:)"    == "CONST spair\<cdot>x\<cdot>y"

translations
  "\<Lambda>(CONST spair\<cdot>x\<cdot>y). t" == "CONST ssplit\<cdot>(\<Lambda> x y. t)"

subsection {* Case analysis *}

lemma spair_Abs_Sprod:
  "(:a, b:) = Abs_Sprod <strictify\<cdot>(\<Lambda> b. a)\<cdot>b, strictify\<cdot>(\<Lambda> a. b)\<cdot>a>"
apply (unfold spair_def)
apply (simp add: cont_Abs_Sprod spair_lemma)
done

lemma Exh_Sprod2:
  "z = \<bottom> \<or> (\<exists>a b. z = (:a, b:) \<and> a \<noteq> \<bottom> \<and> b \<noteq> \<bottom>)"
apply (rule_tac x=z in Abs_Sprod_cases)
apply (simp add: Sprod_def)
apply (erule disjE)
apply (simp add: Abs_Sprod_strict)
apply (rule disjI2)
apply (rule_tac x="cfst\<cdot>y" in exI)
apply (rule_tac x="csnd\<cdot>y" in exI)
apply (simp add: spair_Abs_Sprod Abs_Sprod_inject spair_lemma)
apply (simp add: surjective_pairing_Cprod2)
done

lemma sprodE:
  "\<lbrakk>p = \<bottom> \<Longrightarrow> Q; \<And>x y. \<lbrakk>p = (:x, y:); x \<noteq> \<bottom>; y \<noteq> \<bottom>\<rbrakk> \<Longrightarrow> Q\<rbrakk> \<Longrightarrow> Q"
by (cut_tac z=p in Exh_Sprod2, auto)

subsection {* Properties of @{term spair} *}

lemma spair_strict1 [simp]: "(:\<bottom>, y:) = \<bottom>"
by (simp add: spair_Abs_Sprod strictify_conv_if cpair_strict Abs_Sprod_strict)

lemma spair_strict2 [simp]: "(:x, \<bottom>:) = \<bottom>"
by (simp add: spair_Abs_Sprod strictify_conv_if cpair_strict Abs_Sprod_strict)

lemma spair_strict: "x = \<bottom> \<or> y = \<bottom> \<Longrightarrow> (:x, y:) = \<bottom>"
by auto

lemma spair_strict_rev: "(:x, y:) \<noteq> \<bottom> \<Longrightarrow> x \<noteq> \<bottom> \<and> y \<noteq> \<bottom>"
by (erule contrapos_np, auto)

lemma spair_defined [simp]: 
  "\<lbrakk>x \<noteq> \<bottom>; y \<noteq> \<bottom>\<rbrakk> \<Longrightarrow> (:x, y:) \<noteq> \<bottom>"
by (simp add: spair_Abs_Sprod Abs_Sprod_defined Sprod_def)

lemma spair_defined_rev: "(:x, y:) = \<bottom> \<Longrightarrow> x = \<bottom> \<or> y = \<bottom>"
by (erule contrapos_pp, simp)

lemma spair_eq:
  "\<lbrakk>x \<noteq> \<bottom>; y \<noteq> \<bottom>\<rbrakk> \<Longrightarrow> ((:x, y:) = (:a, b:)) = (x = a \<and> y = b)"
apply (simp add: spair_Abs_Sprod)
apply (simp add: Abs_Sprod_inject [OF _ spair_lemma] Sprod_def)
apply (simp add: strictify_conv_if)
done

lemma spair_inject:
  "\<lbrakk>x \<noteq> \<bottom>; y \<noteq> \<bottom>; (:x, y:) = (:a, b:)\<rbrakk> \<Longrightarrow> x = a \<and> y = b"
by (rule spair_eq [THEN iffD1])

lemma inst_sprod_pcpo2: "UU = (:UU,UU:)"
by simp

lemma Rep_Sprod_spair:
  "Rep_Sprod (:a, b:) = <strictify\<cdot>(\<Lambda> b. a)\<cdot>b, strictify\<cdot>(\<Lambda> a. b)\<cdot>a>"
apply (unfold spair_def)
apply (simp add: cont_Abs_Sprod Abs_Sprod_inverse spair_lemma)
done

lemma compact_spair: "\<lbrakk>compact x; compact y\<rbrakk> \<Longrightarrow> compact (:x, y:)"
by (rule compact_Sprod, simp add: Rep_Sprod_spair strictify_conv_if)

subsection {* Properties of @{term sfst} and @{term ssnd} *}

lemma sfst_strict [simp]: "sfst\<cdot>\<bottom> = \<bottom>"
by (simp add: sfst_def cont_Rep_Sprod Rep_Sprod_strict)

lemma ssnd_strict [simp]: "ssnd\<cdot>\<bottom> = \<bottom>"
by (simp add: ssnd_def cont_Rep_Sprod Rep_Sprod_strict)

lemma sfst_spair [simp]: "y \<noteq> \<bottom> \<Longrightarrow> sfst\<cdot>(:x, y:) = x"
by (simp add: sfst_def cont_Rep_Sprod Rep_Sprod_spair)

lemma ssnd_spair [simp]: "x \<noteq> \<bottom> \<Longrightarrow> ssnd\<cdot>(:x, y:) = y"
by (simp add: ssnd_def cont_Rep_Sprod Rep_Sprod_spair)

lemma sfst_defined_iff [simp]: "(sfst\<cdot>p = \<bottom>) = (p = \<bottom>)"
by (rule_tac p=p in sprodE, simp_all)

lemma ssnd_defined_iff [simp]: "(ssnd\<cdot>p = \<bottom>) = (p = \<bottom>)"
by (rule_tac p=p in sprodE, simp_all)

lemma sfst_defined: "p \<noteq> \<bottom> \<Longrightarrow> sfst\<cdot>p \<noteq> \<bottom>"
by simp

lemma ssnd_defined: "p \<noteq> \<bottom> \<Longrightarrow> ssnd\<cdot>p \<noteq> \<bottom>"
by simp

lemma surjective_pairing_Sprod2: "(:sfst\<cdot>p, ssnd\<cdot>p:) = p"
by (rule_tac p=p in sprodE, simp_all)

lemma less_sprod: "x \<sqsubseteq> y = (sfst\<cdot>x \<sqsubseteq> sfst\<cdot>y \<and> ssnd\<cdot>x \<sqsubseteq> ssnd\<cdot>y)"
apply (simp add: less_Sprod_def sfst_def ssnd_def cont_Rep_Sprod)
apply (rule less_cprod)
done

lemma eq_sprod: "(x = y) = (sfst\<cdot>x = sfst\<cdot>y \<and> ssnd\<cdot>x = ssnd\<cdot>y)"
by (auto simp add: po_eq_conv less_sprod)

lemma spair_less:
  "\<lbrakk>x \<noteq> \<bottom>; y \<noteq> \<bottom>\<rbrakk> \<Longrightarrow> (:x, y:) \<sqsubseteq> (:a, b:) = (x \<sqsubseteq> a \<and> y \<sqsubseteq> b)"
apply (case_tac "a = \<bottom>")
apply (simp add: eq_UU_iff [symmetric])
apply (case_tac "b = \<bottom>")
apply (simp add: eq_UU_iff [symmetric])
apply (simp add: less_sprod)
done


subsection {* Properties of @{term ssplit} *}

lemma ssplit1 [simp]: "ssplit\<cdot>f\<cdot>\<bottom> = \<bottom>"
by (simp add: ssplit_def)

lemma ssplit2 [simp]: "\<lbrakk>x \<noteq> \<bottom>; y \<noteq> \<bottom>\<rbrakk> \<Longrightarrow> ssplit\<cdot>f\<cdot>(:x, y:) = f\<cdot>x\<cdot>y"
by (simp add: ssplit_def)

lemma ssplit3 [simp]: "ssplit\<cdot>spair\<cdot>z = z"
by (rule_tac p=z in sprodE, simp_all)

end
