(*  Title:      HOL/Quadratic_Reciprocity/Gauss.thy
    ID:         $Id$
    Authors:    Jeremy Avigad, David Gray, and Adam Kramer)
*)

header {* Gauss' Lemma *}

theory Gauss imports Euler begin;

locale GAUSS =
  fixes p :: "int"
  fixes a :: "int"
  fixes A :: "int set"
  fixes B :: "int set"
  fixes C :: "int set"
  fixes D :: "int set"
  fixes E :: "int set"
  fixes F :: "int set"

  assumes p_prime: "p \<in> zprime"
  assumes p_g_2: "2 < p"
  assumes p_a_relprime: "~[a = 0](mod p)"
  assumes a_nonzero:    "0 < a"

  defines A_def: "A == {(x::int). 0 < x & x \<le> ((p - 1) div 2)}"
  defines B_def: "B == (%x. x * a) ` A"
  defines C_def: "C == (StandardRes p) ` B"
  defines D_def: "D == C \<inter> {x. x \<le> ((p - 1) div 2)}"
  defines E_def: "E == C \<inter> {x. ((p - 1) div 2) < x}"
  defines F_def: "F == (%x. (p - x)) ` E";

subsection {* Basic properties of p *}

lemma (in GAUSS) p_odd: "p \<in> zOdd";
  by (auto simp add: p_prime p_g_2 zprime_zOdd_eq_grt_2)

lemma (in GAUSS) p_g_0: "0 < p";
  by (insert p_g_2, auto)

lemma (in GAUSS) int_nat: "int (nat ((p - 1) div 2)) = (p - 1) div 2";
  by (insert p_g_2, auto simp add: pos_imp_zdiv_nonneg_iff)

lemma (in GAUSS) p_minus_one_l: "(p - 1) div 2 < p";
  proof -;
    have "p - 1 = (p - 1) div 1" by auto
    then have "(p - 1) div 2 \<le> p - 1"
      apply (rule ssubst) back;
      apply (rule zdiv_mono2)
      by (auto simp add: p_g_0)
    then have "(p - 1) div 2 \<le> p - 1";
      by auto
    then show ?thesis by simp
qed;

lemma (in GAUSS) p_eq: "p = (2 * (p - 1) div 2) + 1";
  apply (insert zdiv_zmult_self2 [of 2 "p - 1"])
by auto

lemma zodd_imp_zdiv_eq: "x \<in> zOdd ==> 2 * (x - 1) div 2 = 2 * ((x - 1) div 2)";
  apply (frule odd_minus_one_even)
  apply (simp add: zEven_def)
  apply (subgoal_tac "2 \<noteq> 0")
  apply (frule_tac b = "2 :: int" and a = "x - 1" in zdiv_zmult_self2)  
by (auto simp add: even_div_2_prop2)

lemma (in GAUSS) p_eq2: "p = (2 * ((p - 1) div 2)) + 1";
  apply (insert p_eq p_prime p_g_2 zprime_zOdd_eq_grt_2 [of p], auto)
by (frule zodd_imp_zdiv_eq, auto)

subsection {* Basic Properties of the Gauss Sets *}

lemma (in GAUSS) finite_A: "finite (A)";
  apply (auto simp add: A_def) 
thm bdd_int_set_l_finite;
  apply (subgoal_tac "{x. 0 < x & x \<le> (p - 1) div 2} \<subseteq> {x. 0 \<le> x & x < 1 + (p - 1) div 2}"); 
by (auto simp add: bdd_int_set_l_finite finite_subset)

lemma (in GAUSS) finite_B: "finite (B)";
  by (auto simp add: B_def finite_A finite_imageI)

lemma (in GAUSS) finite_C: "finite (C)";
  by (auto simp add: C_def finite_B finite_imageI)

lemma (in GAUSS) finite_D: "finite (D)";
  by (auto simp add: D_def finite_Int finite_C)

lemma (in GAUSS) finite_E: "finite (E)";
  by (auto simp add: E_def finite_Int finite_C)

lemma (in GAUSS) finite_F: "finite (F)";
  by (auto simp add: F_def finite_E finite_imageI)

lemma (in GAUSS) C_eq: "C = D \<union> E";
  by (auto simp add: C_def D_def E_def)

lemma (in GAUSS) A_card_eq: "card A = nat ((p - 1) div 2)";
  apply (auto simp add: A_def) 
  apply (insert int_nat)
  apply (erule subst)
  by (auto simp add: card_bdd_int_set_l_le)

lemma (in GAUSS) inj_on_xa_A: "inj_on (%x. x * a) A";
  apply (insert a_nonzero)
by (simp add: A_def inj_on_def)

lemma (in GAUSS) A_res: "ResSet p A";
  apply (auto simp add: A_def ResSet_def) 
  apply (rule_tac m = p in zcong_less_eq) 
  apply (insert p_g_2, auto) 
  apply (subgoal_tac [1-2] "(p - 1) div 2 < p");
by (auto, auto simp add: p_minus_one_l)

lemma (in GAUSS) B_res: "ResSet p B";
  apply (insert p_g_2 p_a_relprime p_minus_one_l)
  apply (auto simp add: B_def) 
  apply (rule ResSet_image)
  apply (auto simp add: A_res) 
  apply (auto simp add: A_def)
  proof -;
    fix x fix y
    assume a: "[x * a = y * a] (mod p)"
    assume b: "0 < x"
    assume c: "x \<le> (p - 1) div 2"
    assume d: "0 < y"
    assume e: "y \<le> (p - 1) div 2"
    from a p_a_relprime p_prime a_nonzero zcong_cancel [of p a x y] 
        have "[x = y](mod p)";
      by (simp add: zprime_imp_zrelprime zcong_def p_g_0 order_le_less) 
    with zcong_less_eq [of x y p] p_minus_one_l 
         order_le_less_trans [of x "(p - 1) div 2" p]
         order_le_less_trans [of y "(p - 1) div 2" p] show "x = y";
      by (simp add: prems p_minus_one_l p_g_0)
qed;

lemma (in GAUSS) SR_B_inj: "inj_on (StandardRes p) B";
  apply (auto simp add: B_def StandardRes_def inj_on_def A_def prems)
  proof -;
    fix x fix y
    assume a: "x * a mod p = y * a mod p"
    assume b: "0 < x"
    assume c: "x \<le> (p - 1) div 2"
    assume d: "0 < y"
    assume e: "y \<le> (p - 1) div 2"
    assume f: "x \<noteq> y"
    from a have "[x * a = y * a](mod p)";
      by (simp add: zcong_zmod_eq p_g_0)
    with p_a_relprime p_prime a_nonzero zcong_cancel [of p a x y] 
        have "[x = y](mod p)";
      by (simp add: zprime_imp_zrelprime zcong_def p_g_0 order_le_less) 
    with zcong_less_eq [of x y p] p_minus_one_l 
         order_le_less_trans [of x "(p - 1) div 2" p]
         order_le_less_trans [of y "(p - 1) div 2" p] have "x = y";
      by (simp add: prems p_minus_one_l p_g_0)
    then have False;
      by (simp add: f)
    then show "a = 0";
      by simp
qed;

lemma (in GAUSS) inj_on_pminusx_E: "inj_on (%x. p - x) E";
  apply (auto simp add: E_def C_def B_def A_def)
  apply (rule_tac g = "%x. -1 * (x - p)" in inj_on_inverseI);
by auto

lemma (in GAUSS) A_ncong_p: "x \<in> A ==> ~[x = 0](mod p)";
  apply (auto simp add: A_def)
  apply (frule_tac m = p in zcong_not_zero)
  apply (insert p_minus_one_l)
by auto

lemma (in GAUSS) A_greater_zero: "x \<in> A ==> 0 < x";
  by (auto simp add: A_def)

lemma (in GAUSS) B_ncong_p: "x \<in> B ==> ~[x = 0](mod p)";
  apply (auto simp add: B_def)
  apply (frule A_ncong_p) 
  apply (insert p_a_relprime p_prime a_nonzero)
  apply (frule_tac a = x and b = a in zcong_zprime_prod_zero_contra)
by (auto simp add: A_greater_zero)

lemma (in GAUSS) B_greater_zero: "x \<in> B ==> 0 < x";
  apply (insert a_nonzero)
by (auto simp add: B_def mult_pos A_greater_zero)

lemma (in GAUSS) C_ncong_p: "x \<in> C ==>  ~[x = 0](mod p)";
  apply (auto simp add: C_def)
  apply (frule B_ncong_p)
  apply (subgoal_tac "[x = StandardRes p x](mod p)");
  defer; apply (simp add: StandardRes_prop1)
  apply (frule_tac a = x and b = "StandardRes p x" and c = 0 in zcong_trans)
by auto

lemma (in GAUSS) C_greater_zero: "y \<in> C ==> 0 < y";
  apply (auto simp add: C_def)
  proof -;
    fix x;
    assume a: "x \<in> B";
    from p_g_0 have "0 \<le> StandardRes p x";
      by (simp add: StandardRes_lbound)
    moreover have "~[x = 0] (mod p)";
      by (simp add: a B_ncong_p)
    then have "StandardRes p x \<noteq> 0";
      by (simp add: StandardRes_prop3)
    ultimately show "0 < StandardRes p x";
      by (simp add: order_le_less)
qed;

lemma (in GAUSS) D_ncong_p: "x \<in> D ==> ~[x = 0](mod p)";
  by (auto simp add: D_def C_ncong_p)

lemma (in GAUSS) E_ncong_p: "x \<in> E ==> ~[x = 0](mod p)";
  by (auto simp add: E_def C_ncong_p)

lemma (in GAUSS) F_ncong_p: "x \<in> F ==> ~[x = 0](mod p)";
  apply (auto simp add: F_def) 
  proof -;
    fix x assume a: "x \<in> E" assume b: "[p - x = 0] (mod p)"
    from E_ncong_p have "~[x = 0] (mod p)";
      by (simp add: a)
    moreover from a have "0 < x";
      by (simp add: a E_def C_greater_zero)
    moreover from a have "x < p";
      by (auto simp add: E_def C_def p_g_0 StandardRes_ubound)
    ultimately have "~[p - x = 0] (mod p)";
      by (simp add: zcong_not_zero)
    from this show False by (simp add: b)
qed;

lemma (in GAUSS) F_subset: "F \<subseteq> {x. 0 < x & x \<le> ((p - 1) div 2)}";
  apply (auto simp add: F_def E_def) 
  apply (insert p_g_0)
  apply (frule_tac x = xa in StandardRes_ubound)
  apply (frule_tac x = x in StandardRes_ubound)
  apply (subgoal_tac "xa = StandardRes p xa")
  apply (auto simp add: C_def StandardRes_prop2 StandardRes_prop1)
  proof -;
    from zodd_imp_zdiv_eq p_prime p_g_2 zprime_zOdd_eq_grt_2 have 
        "2 * (p - 1) div 2 = 2 * ((p - 1) div 2)";
      by simp
    with p_eq2 show " !!x. [| (p - 1) div 2 < StandardRes p x; x \<in> B |]
         ==> p - StandardRes p x \<le> (p - 1) div 2";
      by simp
qed;

lemma (in GAUSS) D_subset: "D \<subseteq> {x. 0 < x & x \<le> ((p - 1) div 2)}";
  by (auto simp add: D_def C_greater_zero)

lemma (in GAUSS) F_eq: "F = {x. \<exists>y \<in> A. ( x = p - (StandardRes p (y*a)) & (p - 1) div 2 < StandardRes p (y*a))}";
  by (auto simp add: F_def E_def D_def C_def B_def A_def)

lemma (in GAUSS) D_eq: "D = {x. \<exists>y \<in> A. ( x = StandardRes p (y*a) & StandardRes p (y*a) \<le> (p - 1) div 2)}";
  by (auto simp add: D_def C_def B_def A_def)

lemma (in GAUSS) D_leq: "x \<in> D ==> x \<le> (p - 1) div 2";
  by (auto simp add: D_eq)

lemma (in GAUSS) F_ge: "x \<in> F ==> x \<le> (p - 1) div 2";
  apply (auto simp add: F_eq A_def)
  proof -;
    fix y;
    assume "(p - 1) div 2 < StandardRes p (y * a)";
    then have "p - StandardRes p (y * a) < p - ((p - 1) div 2)";
      by arith
    also from p_eq2 have "... = 2 * ((p - 1) div 2) + 1 - ((p - 1) div 2)"; 
      by (rule subst, auto)
    also; have "2 * ((p - 1) div 2) + 1 - (p - 1) div 2 = (p - 1) div 2 + 1";
      by arith
    finally show "p - StandardRes p (y * a) \<le> (p - 1) div 2";
      by (insert zless_add1_eq [of "p - StandardRes p (y * a)" 
          "(p - 1) div 2"],auto);
qed;

lemma (in GAUSS) all_A_relprime: "\<forall>x \<in> A. zgcd(x,p) = 1";
  apply (insert p_prime p_minus_one_l)
by (auto simp add: A_def zless_zprime_imp_zrelprime)

lemma (in GAUSS) A_prod_relprime: "zgcd((setprod id A),p) = 1";
  by (insert all_A_relprime finite_A, simp add: all_relprime_prod_relprime)

subsection {* Relationships Between Gauss Sets *}

lemma (in GAUSS) B_card_eq_A: "card B = card A";
  apply (insert finite_A)
by (simp add: finite_A B_def inj_on_xa_A card_image)

lemma (in GAUSS) B_card_eq: "card B = nat ((p - 1) div 2)";
  by (auto simp add: B_card_eq_A A_card_eq)

lemma (in GAUSS) F_card_eq_E: "card F = card E";
  apply (insert finite_E)
by (simp add: F_def inj_on_pminusx_E card_image)

lemma (in GAUSS) C_card_eq_B: "card C = card B";
  apply (insert finite_B)
  apply (subgoal_tac "inj_on (StandardRes p) B");
  apply (simp add: B_def C_def card_image)
  apply (rule StandardRes_inj_on_ResSet)
by (simp add: B_res)

lemma (in GAUSS) D_E_disj: "D \<inter> E = {}";
  by (auto simp add: D_def E_def)

lemma (in GAUSS) C_card_eq_D_plus_E: "card C = card D + card E";
  by (auto simp add: C_eq card_Un_disjoint D_E_disj finite_D finite_E)

lemma (in GAUSS) C_prod_eq_D_times_E: "setprod id E * setprod id D = setprod id C";
  apply (insert D_E_disj finite_D finite_E C_eq)
  apply (frule setprod_Un_disjoint [of D E id])
by auto

lemma (in GAUSS) C_B_zcong_prod: "[setprod id C = setprod id B] (mod p)";
  apply (auto simp add: C_def)
  apply (insert finite_B SR_B_inj) 
  apply (frule_tac f1 = "StandardRes p" in setprod_reindex_id[THEN sym], auto)
  apply (rule setprod_same_function_zcong)
by (auto simp add: StandardRes_prop1 zcong_sym p_g_0)

lemma (in GAUSS) F_Un_D_subset: "(F \<union> D) \<subseteq> A";
  apply (rule Un_least)
by (auto simp add: A_def F_subset D_subset)

lemma two_eq: "2 * (x::int) = x + x";
  by arith

lemma (in GAUSS) F_D_disj: "(F \<inter> D) = {}";
  apply (simp add: F_eq D_eq)
  apply (auto simp add: F_eq D_eq)
  proof -;
    fix y; fix ya;
    assume "p - StandardRes p (y * a) = StandardRes p (ya * a)";
    then have "p = StandardRes p (y * a) + StandardRes p (ya * a)";
      by arith
    moreover have "p dvd p";
      by auto
    ultimately have "p dvd (StandardRes p (y * a) + StandardRes p (ya * a))";
      by auto
    then have a: "[StandardRes p (y * a) + StandardRes p (ya * a) = 0] (mod p)";
      by (auto simp add: zcong_def)
    have "[y * a = StandardRes p (y * a)] (mod p)";
      by (simp only: zcong_sym StandardRes_prop1)
    moreover have "[ya * a = StandardRes p (ya * a)] (mod p)";
      by (simp only: zcong_sym StandardRes_prop1)
    ultimately have "[y * a + ya * a = 
        StandardRes p (y * a) + StandardRes p (ya * a)] (mod p)";
      by (rule zcong_zadd)
    with a have "[y * a + ya * a = 0] (mod p)";
      apply (elim zcong_trans)
      by (simp only: zcong_refl)
    also have "y * a + ya * a = a * (y + ya)";
      by (simp add: zadd_zmult_distrib2 zmult_commute)
    finally have "[a * (y + ya) = 0] (mod p)";.;
    with p_prime a_nonzero zcong_zprime_prod_zero [of p a "y + ya"]
        p_a_relprime
        have a: "[y + ya = 0] (mod p)";
      by auto
    assume b: "y \<in> A" and c: "ya: A";
    with A_def have "0 < y + ya";
      by auto
    moreover from b c A_def have "y + ya \<le> (p - 1) div 2 + (p - 1) div 2";
      by auto 
    moreover from b c p_eq2 A_def have "y + ya < p";
      by auto
    ultimately show False;
      apply simp
      apply (frule_tac m = p in zcong_not_zero)
      by (auto simp add: a)
qed;

lemma (in GAUSS) F_Un_D_card: "card (F \<union> D) = nat ((p - 1) div 2)";
  apply (insert F_D_disj finite_F finite_D)
  proof -;
    have "card (F \<union> D) = card E + card D";
      by (auto simp add: finite_F finite_D F_D_disj 
                         card_Un_disjoint F_card_eq_E)
    then have "card (F \<union> D) = card C";
      by (simp add: C_card_eq_D_plus_E)
    from this show "card (F \<union> D) = nat ((p - 1) div 2)"; 
      by (simp add: C_card_eq_B B_card_eq)
qed;

lemma (in GAUSS) F_Un_D_eq_A: "F \<union> D = A";
  apply (insert finite_A F_Un_D_subset A_card_eq F_Un_D_card) 
by (auto simp add: card_seteq)

lemma (in GAUSS) prod_D_F_eq_prod_A: 
    "(setprod id D) * (setprod id F) = setprod id A";
  apply (insert F_D_disj finite_D finite_F)
  apply (frule setprod_Un_disjoint [of F D id])
by (auto simp add: F_Un_D_eq_A)

lemma (in GAUSS) prod_F_zcong:
    "[setprod id F = ((-1) ^ (card E)) * (setprod id E)] (mod p)"
  proof -
    have "setprod id F = setprod id (op - p ` E)"
      by (auto simp add: F_def)
    then have "setprod id F = setprod (op - p) E"
      apply simp
      apply (insert finite_E inj_on_pminusx_E)
      by (frule_tac f = "op - p" in setprod_reindex_id, auto)
    then have one: 
      "[setprod id F = setprod (StandardRes p o (op - p)) E] (mod p)"
      apply simp
      apply (insert p_g_0 finite_E)
      by (auto simp add: StandardRes_prod)
    moreover have a: "\<forall>x \<in> E. [p - x = 0 - x] (mod p)"
      apply clarify
      apply (insert zcong_id [of p])
      by (rule_tac a = p and m = p and c = x and d = x in zcong_zdiff, auto)
    moreover have b: "\<forall>x \<in> E. [StandardRes p (p - x) = p - x](mod p)"
      apply clarify
      by (simp add: StandardRes_prop1 zcong_sym)
    moreover have "\<forall>x \<in> E. [StandardRes p (p - x) = - x](mod p)"
      apply clarify
      apply (insert a b)
      by (rule_tac b = "p - x" in zcong_trans, auto)
    ultimately have c:
      "[setprod (StandardRes p o (op - p)) E = setprod (uminus) E](mod p)"
      apply simp
      apply (insert finite_E p_g_0)
      by (rule setprod_same_function_zcong [of E "StandardRes p o (op - p)"
                                                     uminus p], auto)
    then have two: "[setprod id F = setprod (uminus) E](mod p)"
      apply (insert one c)
      by (rule zcong_trans [of "setprod id F" 
                               "setprod (StandardRes p o op - p) E" p
                               "setprod uminus E"], auto) 
    also have "setprod uminus E = (setprod id E) * (-1)^(card E)" 
      apply (insert finite_E)
      by (induct set: Finites, auto)
    then have "setprod uminus E = (-1) ^ (card E) * (setprod id E)"
      by (simp add: zmult_commute)
    with two show ?thesis
      by simp
qed

subsection {* Gauss' Lemma *}

lemma (in GAUSS) aux: "setprod id A * -1 ^ card E * a ^ card A * -1 ^ card E = setprod id A * a ^ card A"
  by (auto simp add: finite_E neg_one_special)

theorem (in GAUSS) pre_gauss_lemma:
    "[a ^ nat((p - 1) div 2) = (-1) ^ (card E)] (mod p)"
  proof -
    have "[setprod id A = setprod id F * setprod id D](mod p)"
      by (auto simp add: prod_D_F_eq_prod_A zmult_commute)
    then have "[setprod id A = ((-1)^(card E) * setprod id E) * 
        setprod id D] (mod p)"
      apply (rule zcong_trans)
      by (auto simp add: prod_F_zcong zcong_scalar)
    then have "[setprod id A = ((-1)^(card E) * setprod id C)] (mod p)"
      apply (rule zcong_trans)
      apply (insert C_prod_eq_D_times_E, erule subst)
      by (subst zmult_assoc, auto)
    then have "[setprod id A = ((-1)^(card E) * setprod id B)] (mod p)"
      apply (rule zcong_trans)
      by (simp add: C_B_zcong_prod zcong_scalar2)
    then have "[setprod id A = ((-1)^(card E) *
        (setprod id ((%x. x * a) ` A)))] (mod p)"
      by (simp add: B_def)
    then have "[setprod id A = ((-1)^(card E) * (setprod (%x. x * a) A))] 
        (mod p)"
      apply (rule zcong_trans)
      by (simp add: finite_A inj_on_xa_A setprod_reindex_id zcong_scalar2)
    moreover have "setprod (%x. x * a) A = 
        setprod (%x. a) A * setprod id A"
      by (insert finite_A, induct set: Finites, auto)
    ultimately have "[setprod id A = ((-1)^(card E) * (setprod (%x. a) A * 
        setprod id A))] (mod p)"
      by simp 
    then have "[setprod id A = ((-1)^(card E) * a^(card A) * 
        setprod id A)](mod p)"
      apply (rule zcong_trans)
      by (simp add: zcong_scalar2 zcong_scalar finite_A setprod_constant
        zmult_assoc)
    then have a: "[setprod id A * (-1)^(card E) = 
        ((-1)^(card E) * a^(card A) * setprod id A * (-1)^(card E))](mod p)"
      by (rule zcong_scalar)
    then have "[setprod id A * (-1)^(card E) = setprod id A * 
        (-1)^(card E) * a^(card A) * (-1)^(card E)](mod p)"
      apply (rule zcong_trans)
      by (simp add: a mult_commute mult_left_commute)
    then have "[setprod id A * (-1)^(card E) = setprod id A * 
        a^(card A)](mod p)"
      apply (rule zcong_trans)
      by (simp add: aux)
    with this zcong_cancel2 [of p "setprod id A" "-1 ^ card E" "a ^ card A"]
         p_g_0 A_prod_relprime have "[-1 ^ card E = a ^ card A](mod p)"
       by (simp add: order_less_imp_le)
    from this show ?thesis
      by (simp add: A_card_eq zcong_sym)
qed

theorem (in GAUSS) gauss_lemma: "(Legendre a p) = (-1) ^ (card E)"
proof -
  from Euler_Criterion p_prime p_g_2 have
    "[(Legendre a p) = a^(nat (((p) - 1) div 2))] (mod p)"
    by auto
  moreover note pre_gauss_lemma
  ultimately have "[(Legendre a p) = (-1) ^ (card E)] (mod p)"
    by (rule zcong_trans)
  moreover from p_a_relprime have "(Legendre a p) = 1 | (Legendre a p) = (-1)"
    by (auto simp add: Legendre_def)
  moreover have "(-1::int) ^ (card E) = 1 | (-1::int) ^ (card E) = -1"
    by (rule neg_one_power)
  ultimately show ?thesis
    by (auto simp add: p_g_2 one_not_neg_one_mod_m zcong_sym)
qed

end